cedar-lean/Cedar/Thm/Data/List/Canonical.lean
@@ -46,6 +46,46 @@ theorem insertCanonical_not_nil [DecidableEq β] [LT β] [DecidableLT β] (f : �
     split at h <;> try trivial
     split at h <;> trivial
 
+theorem insertCanonical_exists [LT β] [Cedar.Data.StrictLT β] [DecidableLT β]
+  {f : α → β} {xs : List α} (x : α) :
+  x ∈ List.insertCanonical f x xs
+:= by
+  induction xs
+  case nil => simp [List.insertCanonical]
+  case cons head tail ih =>
+    simp [List.insertCanonical]
+    split; any_goals simp
+    split; any_goals simp
+    apply Or.inr ih
+
+theorem insertCanonical_new
+  [LT β] [Cedar.Data.StrictLT β] [DecidableLT β] [DecidableEq β]
+  {f : α → β} {xs : List α} {x : α} {y : α}
+  (hexists : y ∈ xs)
+  (hneq : f x ≠ f y) :
+  y ∈ List.insertCanonical f x xs
+:= by
+  induction xs
+
+  case nil => simp at hexists
+
+  case cons hd tl ih =>
+    simp [List.insertCanonical]
+    split
+    simp [hexists]
+    split
+    · simp at hexists
+      cases hexists
+      case _ hy => simp [hy]
+      case _ hy => simp [ih hy]
+    · simp at hexists
+      cases hexists
+      case _ hlt hgt hy =>
+        simp [← hy] at hlt hgt
+        have hltgt := StrictLT.connected (f x) (f y) hneq
+        cases hltgt <;> contradiction
+      case _ hy => simp [hy]
+
 theorem insertCanonical_sortedBy [LT β] [StrictLT β] [DecidableLT β] {f : α → β} {xs : List α} (x : α) :
   SortedBy f xs →
   SortedBy f (insertCanonical f x xs)
